new style

ftvsdjit.dfy
@@ -33,13 +33,16 @@ ensures forall i : char :: i in res.vs ==> res.vs[i].val == 0
 
 ghost method djitStep (ds : DjitState, op : Op, size : nat) returns (res : opt<DjitState>)
 requires size > 0
-requires op.loc in ds.vs
-requires op.tid in ds.ts
 requires forall j : int :: j in ds.ts ==> |ds.ts[j]| == size 
 requires forall j : char :: j in ds.vs ==> |ds.vs[j]| == size 
-requires forall j : int :: j in ds.ts ==> |ds.ts[j]| == size
-//ensures (res.Just?) ==> (forall i : int :: 0 <= i < size ==> ds.vs[op.loc][i] <= ds.ts[op.tid][i])
-ensures (res.Just?) ==> (forall i : int :: 0 <= i < size ==> ds.vs[op.loc][i] <= ds.ts[op.tid][i])
+requires op.loc in ds.vs
+requires op.tid in ds.ts
+requires 0 <= op.tid < size
+ensures (res.Just?) ==> forall j : int :: j in res.value.ts ==> |res.value.ts[j]| == size 
+ensures (res. Just?) ==> forall j : char :: j in res.value.vs ==> |res.value.vs[j]| == size 
+ensures (res.Just?) ==> op.loc in res.value.vs
+ensures (res.Just?) ==> op.tid in res.value.ts
+ensures (res.Just?) ==> (forall i : int :: 0 <= i < size ==> res.value.vs[op.loc][i] <= res.value.ts[op.tid][i])
 ensures (res == Nothing) ==> (exists i : int :: 0 <= i < size && ds.vs[op.loc][i] > ds.ts[op.tid][i])
 {
 	
@@ -53,7 +56,23 @@ ensures (res == Nothing) ==> (exists i : int :: 0 <= i < size && ds.vs[op.loc][i
 		}
 		else
 		{
-			res :=  Just(ds);
+			//ts state
+			var tmapTemp := ds.ts;
+			var tvcTemp := tmapTemp[tid];
+			var tvalTemp := tvcTemp[tid];
+			tvcTemp := tvcTemp[tid := tvalTemp];
+			tmapTemp := tmapTemp[tid := tvcTemp];
+			
+			// vs state
+			var vmapTemp := ds.vs;
+			var vvcTemp := vmapTemp[loc];
+			var vvalTemp := vvcTemp[tid];
+			vvcTemp := vvcTemp[tid := vvalTemp];
+			vmapTemp := vmapTemp[loc := vvcTemp];
+		
+			// make new djit state
+			var dsTemp := DjitState(tmapTemp, vmapTemp);
+			res :=  Just(dsTemp);
 		}
 	}
 }
@@ -89,29 +108,77 @@ ghost method ftStep (fs : FtState, op : Op, size : nat) returns (res : opt<FtSta
 requires size > 0
 requires op.loc in fs.vs
 requires op.tid in fs.ts
+requires 0 <= op.tid < size
 requires forall i : char :: i in fs.vs ==> 0 <= fs.vs[i].tid < size
 requires forall j : int :: j in fs.ts ==> |fs.ts[j]| == size
 requires 0 <= fs.vs[op.loc].tid < size
-requires forall i : int :: 0 <= i < |fs.ts[op.tid]| && i != fs.vs[op.loc].tid ==> fs.vs[op.loc].val <= fs.ts[op.tid][i]
+requires fs.vs[op.loc].tid in fs.ts
+requires fs.vs[op.loc].val <= fs.ts[op.tid][fs.vs[op.loc].tid]
 //ensures (res.Just?) ==> (forall i : int :: 0 <= i < |fs.ts[op.tid]| ==> fs.vs[op.loc].val <= fs.ts[op.tid][i])
-ensures (res.Just?) ==> (forall i : int :: 0 <= i < |fs.ts[op.tid]| ==> fs.vs[op.loc].val <= fs.ts[op.tid][i])
+ensures (res.Just?) ==> forall j : int :: j in res.value.ts ==> |res.value.ts[j]| == size 
+ensures (res.Just?) ==> op.loc in res.value.vs
+ensures (res.Just?) ==> op.tid in res.value.ts
+ensures (res.Just?) ==> res.value.vs[op.loc].tid in res.value.ts
+ensures (res.Just?) ==> 0 <= res.value.vs[op.loc].tid < size
 ensures (res == Nothing) ==> (exists i : int :: 0 <= i < size && fs.vs[op.loc].val > fs.ts[op.tid][i]);
+ensures(res.Just?) ==> fs.vs[op.loc].val <= fs.ts[op.tid][fs.vs[op.loc].tid];
+ensures (res == Nothing) ==> fs.vs[op.loc].val <= fs.ts[op.tid][fs.vs[op.loc].tid];
 {
 	
 	match op
 	case Write(tid, loc) => 
 	{
+
+		
 		var eid := fs.vs[loc].tid;
+		
 		if(fs.vs[loc].val > fs.ts[tid][eid])
 		{
 			res := Nothing;
 		}
 		else
 		{
-			res := Just(fs);
+			var tmapTemp := fs.ts;
+			var tvcTemp := tmapTemp[tid];
+			var tvalTemp := tvcTemp[tid] + 1;
+			tvcTemp := tvcTemp[tid := tvalTemp];
+			tmapTemp := tmapTemp[tid := tvcTemp];
+
+			//fs
+			var emapTemp := fs.vs;
+			var evalTemp := tmapTemp[tid][tid];
+			var eTemp := Epoch(tid, evalTemp);
+			emapTemp := emapTemp[loc := eTemp];
+			var fsTemp := FtState(tmapTemp, emapTemp);
+			assert fsTemp.vs[loc].val == fsTemp.ts[tid][tid];
+			res := Just(fsTemp);
 		}
 	}
+	
 }
+		/*if(fs.vs[loc].val > fs.ts[tid][eid])
+		{
+			res := Nothing;
+		}
+		else
+		{*/
+			//ts
+			/*var tmapTemp := fs.ts;
+			var tvcTemp := tmapTemp[tid];
+			var tvalTemp := tvcTemp[tid] + 1;
+			tvcTemp := tvcTemp[tid := tvalTemp];
+			tmapTemp := tmapTemp[tid := tvcTemp];
+
+			//fs
+			var emapTemp := fs.vs;
+			var evalTemp := tmapTemp[tid][tid];
+			var eTemp := Epoch(tid, evalTemp);
+			emapTemp := emapTemp[loc := eTemp];
+			var fsTemp := FtState(tmapTemp, emapTemp);
+			assert fsTemp.vs[loc].val == fsTemp.ts[tid][tid];
+			assert forall i : int :: 0 <= i < size ==> fsTemp.vs[op.loc].val <= fsTemp.ts[op.tid][i];*/
+			
+	
 
 /*function ftstep_func(fs : FtState, size : nat) : opt<FtState>
 {
@@ -124,11 +191,15 @@ function djitstep_func(ds : FtState, size : nat) : opt<DjitState>
 
 lemma ftstep_equals_djitstep(fs : FtState, ds : DjitState, op :  Op, size :nat)
 requires size > 0
+requires 0 <= op.tid < size 
 requires op.loc in fs.vs
 requires op.tid in fs.ts
 requires forall i : char :: i in fs.vs ==> 0 <= fs.vs[i].tid < size
 requires forall j : int :: j in fs.ts ==> |fs.ts[j]| == size
 requires forall i : int :: 0 <= i < |fs.ts[op.tid]| && i != fs.vs[op.loc].tid ==> fs.vs[op.loc].val <= fs.ts[op.tid][i]
+requires fs.vs[op.loc].tid in fs.ts
+requires 0 <= fs.vs[op.loc].tid < size
+requires fs.vs[op.loc].val <= fs.ts[op.tid][fs.vs[op.loc].tid]
 requires op.loc in ds.vs
 requires op.tid in ds.ts
 requires forall j : int :: j in ds.ts ==> |ds.ts[j]| == size 
@@ -143,19 +214,24 @@ requires (fs.vs[op.loc].val == ds.vs[op.loc][fs.vs[op.loc].tid]);
 	assert ft == Nothing <==> djit == Nothing;
 }
 
-
-
-/*ghost method ft( trace : Trace, size : nat, vars : seq<char>) returns ( res : bool )
+/*lemma maxIdinTrace(trace : Trace)
 requires |trace| > 0
-requires size > 0
-requires |vars| > 0
-requires forall i,j : int :: 0 <= i < j < |vars| ==> vars[i] != vars[j]
-requires forall i : int :: 0 <= i < |trace| ==> 0 <= trace[i].tid < size
-requires forall i : int :: 0 <= i < |trace| ==> trace[i].loc in vars
-requires forall c : char :: c in vars <==> c in getVars(trace,[])
 {
-	var fts := ftStart(size,vars);
-	var ftres := ftStep(fts,trace[0],size);
+		var max := getMaxId(trace);
+		assert max in getIds(trace);
+}*/
+
+
+ghost method ft( trace : Trace, numberOfThreads : nat) returns ( res : bool )
+requires |trace| > 0
+requires numberOfThreads > 0
+requires forall i : int :: 0 <= i < |trace| ==> 0 <= trace[i].tid < numberOfThreads
+requires getMaxIdF(trace, 0, 0) in getIds(trace);
+{
+	var vars := getVarsM(trace);
+	var maxId := getMaxIdF(trace, 0, 0);
+	var fts := ftStart(numberOfThreads,vars);
+	var ftres := ftStep(fts,trace[0],numberOfThreads);
 	if(ftres.Just?)
 	{
 		res := false;
@@ -164,34 +240,29 @@ requires forall c : char :: c in vars <==> c in getVars(trace,[])
 	{
 		res := true;
 	}
-	//var c := findLargestEpoch(lmap[vars[0]]);
-	//var q := lmap[vars[0]].epoch;
-	//assert c.tid == 0;
-	//var resft := false;
-	//var resdjit := false;
-}*/
+}
 
-ghost method djitStart(size : nat, vars : seq<char>) returns (res : DjitState)
-requires size > 0
+ghost method djitStart(numberOfThreads : nat, vars : seq<char>) returns (res : DjitState)
+requires numberOfThreads > 0
 requires |vars| > 0
 requires forall i,j : int :: 0 <= i < j < |vars| ==> vars[i] != vars[j]
-ensures forall i:int :: i in res.ts <==> 0 <= i < size
-ensures forall j : int :: 0 <= j < size ==> |res.ts[j]| == size
-ensures forall j : char :: j in res.vs ==> 0 < |res.vs[j]| == size
-ensures forall j : int :: 0 <= j < size ==> forall i : int :: 0 <= i < size ==> res.ts[j][i] == 0
+ensures forall i:int :: i in res.ts <==> 0 <= i < numberOfThreads
+ensures forall j : int :: 0 <= j < numberOfThreads ==> |res.ts[j]| == numberOfThreads
+ensures forall j : char :: j in res.vs ==> 0 < |res.vs[j]| == numberOfThreads
+ensures forall j : int :: 0 <= j < numberOfThreads ==> forall i : int :: 0 <= i < numberOfThreads ==> res.ts[j][i] == 0
 ensures forall i:char :: i in res.vs ==> i in vars
 ensures forall i : char :: i in vars ==> i in res.vs
-ensures forall i : int :: 0 <= i < size ==> forall j : int :: 0 <= j < size ==> res.ts[i][j] == 0
+ensures forall i : int :: 0 <= i < numberOfThreads ==> forall j : int :: 0 <= j < numberOfThreads ==> res.ts[i][j] == 0
 ensures forall i : char :: i in res.vs ==> forall j : int :: 0 <= j < |res.vs[i]| ==> res.vs[i][j] == 0
 {
-	var tmap := initThreadMap(size);
-	var vmap := initVarsMap(vars,size);
+	var tmap := initThreadMap(numberOfThreads);
+	var vmap := initVarsMap(vars,numberOfThreads);
 	res := DjitState(tmap,vmap);
 }
 
-ghost method initEpochMap(vars: seq<char>, size : nat) returns (res : EpochMap)
+ghost method initEpochMap(vars: seq<char>, numberOfThreads : nat) returns (res : EpochMap)
 requires |vars| > 0
-requires size > 0
+requires numberOfThreads > 0
 requires forall i,j :: 0 <= i < j < |vars| ==> vars[i] != vars[j]
 //requires forall i:int :: i in tmap ==> |tmap[i].vc| == size;
 //requires |tmap| == size
@@ -199,7 +270,7 @@ requires forall i,j :: 0 <= i < j < |vars| ==> vars[i] != vars[j]
 //requires forall i :int :: 0 <= i < size ==> forall j : int :: 0 <= j < size ==> tmap[i].vc[j] == 0;
 //ensures forall i:char :: i in res ==> |res[i].vc| == size;
 ensures forall i:char :: i in res ==> i in vars
-ensures forall i : char :: i in res ==> 0 <= res[i].tid < size
+ensures forall i : char :: i in res ==> 0 <= res[i].tid < numberOfThreads
 //ensures forall i : char :: i in res ==> prop_largest_epoch(res[i]) == true
 //ensures forall i : char :: i in res ==> forall j :int :: 0 <= j < |res[i].vc| ==> res[i].vc[j] == 0
 ensures forall i : char :: i in vars ==> i in res
@@ -215,7 +286,7 @@ ensures forall i : char :: i in res ==> res[i].val == 0
 	invariant forall i,j :: 0 <= i < j < |vars| ==> vars[i] != vars[j]
 	invariant forall i:char :: i in res ==> i in vars
 	invariant forall i: int :: 0 <= i < j ==> vars[i] in res
-	invariant forall i : char :: i in res ==> 0 <= res[i].tid < size
+	invariant forall i : char :: i in res ==> 0 <= res[i].tid < numberOfThreads
 	invariant forall i : char :: i in res ==> res[i].val == 0
 	//invariant forall i : char :: i in res ==> res[i].epoch.val in res[i].vc
 	//invariant forall i : char :: i in res ==> res[i].vc[res[i].epoch.tid] == res[i].epoch.val
@@ -229,22 +300,23 @@ ensures forall i : char :: i in res ==> res[i].val == 0
 	}
 } 
 
-ghost method initThreadMap(size : nat) returns (res : ThreadsMap)
-ensures forall i:int :: i in res ==> |res[i]| == size;
-ensures forall i: int :: i in res ==> forall j : int :: 0 <= j < size ==> res[i][j] == 0
-ensures forall i:int :: i in res <==> 0 <= i < size
-ensures |res| == size
+ghost method initThreadMap(numberOfThreads : nat) returns (res : ThreadsMap)
+ensures forall i:int :: i in res ==> |res[i]| == numberOfThreads;
+ensures forall i: int :: i in res ==> forall j : int :: 0 <= j < numberOfThreads ==> res[i][j] == 0
+ensures forall i:int :: i in res <==> 0 <= i < numberOfThreads
+ensures |res| == numberOfThreads
 {
 	var j := 0;
 	var tmap : ThreadsMap := map[];
-	while( j < size )
-	invariant size >= j >= 0  
-	invariant forall i:int :: i in tmap ==> |tmap[i]| == size;
+	while( j < numberOfThreads )
+	invariant numberOfThreads >= j >= 0  
+	invariant forall i:int :: i in tmap ==> |tmap[i]| == numberOfThreads;
 	invariant |tmap| == j;
 	invariant forall i:int :: i in tmap <==> 0 <= i < j
-	invariant forall i : int :: i in tmap ==> forall j : int :: 0 <= j < size ==> tmap[i][j] == 0
+	invariant forall i : int :: i in tmap ==> forall j : int :: 0 <= j < numberOfThreads ==> tmap[i][j] == 0
 	{
-		var vc := getEmptyVc(size);
+		var vc := getEmptyVc(numberOfThreads);
+		assert j !in tmap;
         tmap := tmap[j := vc];
 		j := j + 1;
 	}
@@ -262,16 +334,16 @@ requires |t| >= 0
 	case Write(id, l) => if( l !in list) then getVars(t[1..], [l] + list) else getVars(t[1..], list)  
 }
 
-ghost method getEmptyVc ( size : nat ) returns ( res : VC )
-requires size > 0
-ensures |res| == size
-ensures forall i : int :: 0 <= i < size ==> res[i] == 0;
+ghost method getEmptyVc ( numberOfThreads : nat ) returns ( res : VC )
+requires numberOfThreads > 0
+ensures |res| == numberOfThreads
+ensures forall i : int :: 0 <= i < numberOfThreads ==> res[i] == 0;
 {
 			var k := 0;
 			res := [];
-			while( k < size)
+			while( k < numberOfThreads)
 			invariant k == |res|
-			invariant size >= k >= 0
+			invariant numberOfThreads >= k >= 0
 			invariant forall i : int :: 0 <= i < k ==> res[i] == 0;
 			
 			{
@@ -280,15 +352,15 @@ ensures forall i : int :: 0 <= i < size ==> res[i] == 0;
 			}
 }
 
-ghost method initVarsMap( vars: seq<char>, size : nat) returns (res : VarsMap)
+ghost method initVarsMap( vars: seq<char>, numberOfThreads : nat) returns (res : VarsMap)
 requires |vars| > 0
-requires size > 0
+requires numberOfThreads > 0
 requires forall i,j :: 0 <= i < j < |vars| ==> vars[i] != vars[j]
 //requires forall i:int :: i in tmap ==> |tmap[i]| == size;
 //requires |tmap| == size
 //requires forall i:int :: i in tmap <==> 0 <= i < size
 //requires forall i :int :: 0 <= i < size ==> forall j : int :: 0 <= j < size ==> tmap[i][j] == 0;
-ensures forall i:char :: i in res ==> |res[i]| == size;
+ensures forall i:char :: i in res ==> |res[i]| == numberOfThreads;
 ensures forall i:char :: i in res ==> i in vars
 //ensures forall i : char :: i in res ==> 0 <= res[i].epoch.tid < size
 //ensures forall i : char :: i in res ==> prop_largest_epoch(res[i]) == true
@@ -306,7 +378,7 @@ ensures forall i : char :: i in vars ==> i in res
 	//WSWinvariant |res| == j
 	invariant 0 <= j <= |vars|
 	invariant forall i,j :: 0 <= i < j < |vars| ==> vars[i] != vars[j]
-	invariant forall i:char :: i in res ==> |res[i]| == size
+	invariant forall i:char :: i in res ==> |res[i]| == numberOfThreads
 	invariant forall i:char :: i in res ==> i in vars
 	invariant forall i: int :: 0 <= i < j ==> vars[i] in res
 	invariant forall i : char :: i in res ==> i in vars
@@ -321,7 +393,7 @@ ensures forall i : char :: i in vars ==> i in res
 	//invariant forall i : char :: i in res ==> res[i].epoch.val == findLargestEpoch(vs,size)
 	{
 		var c:= vars[j];
-		var vc := getEmptyVc(size);
+		var vc := getEmptyVc(numberOfThreads);
 		res := res[c := vc];
 		//assert forall j :int :: 0 <= j < |vc| ==> vc[j] == 0;
 		//assert |vc| == size;
@@ -336,4 +408,75 @@ ensures forall i : char :: i in vars ==> i in res
 		j := j + 1;
 	}
 } 
+
+ghost method getVarsM(trace: Trace) returns (res: seq<char>)
+requires |trace| > 0
+ensures |res| > 0
+ensures forall i : int :: 0 <= i < |trace| ==> trace[i].loc in res
+ensures forall i,j :: 0 <= i < j < |res| ==> res[i] != res[j]
+{
+	var v := trace[0].loc;
+	res := [];
+	res := [v] + res;
+	var i := 0;
+	while( i < |trace| )
+	invariant 0 <= i <= |trace|
+	invariant forall i,j :: 0 <= i < j < |res| ==> res[i] != res[j]
+	invariant forall j : int :: 0 <= j < i ==> trace[j].loc in res 
+	invariant |res| > 0
+	{
+		var step := trace[i];
+		if( step.loc !in res) 
+		{ 
+			res:= [step.loc] + res; 
+		}  
+		i := i + 1;
+	}
+}
+
+function getId(t : Op) : Tid
+{
+	match t
+	case Write(id, l) => id
+}
+
+
+function getIds(t : Trace) : seq<Tid>
+requires |t| >= 0
+{
+	if(|t| == 0) then []
+	else
+	match t[0]
+	case Write(id,l) => [id] + getIds(t[1..])
+}
+
+ghost method getMaxId(t : Trace) returns ( res : Tid)
+requires |t| > 0
+ensures forall j : int :: 0 <= j < |t| ==> res >= t[j].tid
+ensures exists j : int :: 0 <= j < |t| && res == t[j].tid
+{
+	var i := 0;
+	res := t[0].tid;
+	while ( i < |t|)
+	invariant 0 <= i <= |t|
+	invariant forall j : int :: 0 <= j < i ==> res >= t[j].tid
+	invariant exists j : int :: 0 <= j < |t| && res == t[j].tid
+	{
+		if(t[i].tid > res)
+		{
+			res := t[i].tid;
+		}
+		i := i + 1;
+	}
+}
+
+function getMaxIdF(t : Trace, i : nat, max : int) : Tid
+requires |t| > 0
+requires |t| >= i >= 0
+requires max >= 0
+decreases |t| - i
+{
+	if(i == |t|) then max
+	else if (t[i].tid > max) then getMaxIdF(t, i + 1, t[i].tid) else getMaxIdF(t, i + 1, max)
+}
 
