ftvsdjit_functional.dfy
@@ -1,0 +1,134 @@
+datatype Op = Write(tid:int, loc: char)
+datatype opt<T> = Just(value: T) | Nothing
+datatype FtState = FtState(ts : ThreadsMap, vs: EpochMap, ls : VarsMap)
+datatype DjitState = DjitState(ts : ThreadsMap, vs: VarsMap)
+datatype Epoch = Epoch(tid : int, val : int)
+type ThreadsMap = map<int, VC>
+type VarsMap = map<char, VC>
+type EpochMap = map<char, Epoch>
+type Trace = seq<Op>
+type VC = map<int,int>
+
+//The initial state of the fast track algorithm which returns an
+//empty map for each map in the state.
+/*function ftStart(numberOfThreads : nat) : FtState
+requires numberOfThreads > 0
+{
+	var tmap := createThreadsMap(numberOfThreads);
+	assert |tmap| == numberOfThreads;
+	assert forall t : int :: t in tmap ==> |tmap[t]| == numberOfThreads;
+	assert forall t,u : int :: t in tmap && u in tmap && u != t ==> tmap[u][t] < tmap[t][t];
+	var emap := map[];
+	var lmap := map[];
+	//assert 3 == 4;
+	FtState(tmap,emap, lmap)
+}
+
+function createThreadsMap(numberOfThreads : nat) : ThreadsMap
+//ensures forall t : int :: t in createThreadsMap(numberOfThreads) ==> |createThreadsMap(numberOfThreads)[t]| == numberOfThreads
+//ensures |createThreadsMap(numberOfThreads)| == numberOfThreads
+{
+	var v := initThreadMap(numberOfThreads,numberOfThreads);
+	//assert |v| == 3;
+	//assert v[1][1] == v[0][0];
+	assert forall t,u : int :: t in v && u in v && u != t ==> v[u][t] < v[t][t];
+	v
+}
+
+function method initThreadMap(numberOfThreads : nat, const_numberOfThreads : nat) : ThreadsMap
+requires const_numberOfThreads >= numberOfThreads >=0
+ensures forall t : int :: t in initThreadMap(numberOfThreads,const_numberOfThreads) ==> 0 <= t < numberOfThreads
+ensures |initThreadMap(numberOfThreads, const_numberOfThreads)| == numberOfThreads
+ensures forall t : int :: t in initThreadMap(numberOfThreads,const_numberOfThreads) ==> |initThreadMap(numberOfThreads,const_numberOfThreads)[t]| == const_numberOfThreads;
+ensures (var tmap := initThreadMap(numberOfThreads,const_numberOfThreads); forall t : int :: t in tmap ==> tmap[t][t] == 1);
+{
+	if( numberOfThreads == 0) then map[]
+	else var tempMap := initThreadMap(numberOfThreads-1,const_numberOfThreads); tempMap[numberOfThreads-1 := getEmptyVC(numberOfThreads-1,const_numberOfThreads)]
+}
+
+function method getEmptyVC( currId : nat , numberOfThreads : nat) : seq<int>
+requires 0 <= currId 
+ensures |getEmptyVC(currId,numberOfThreads)| == numberOfThreads
+ensures (var m := getEmptyVC(currId,numberOfThreads); |m| >= currId ==> m[currId] == 1)
+{
+	if(numberOfThreads == 0) then []
+	else if(currId == numberOfThreads - 1) then getEmptyVC(currId,numberOfThreads-1)+[1]
+	else getEmptyVC(currId, numberOfThreads-1)+[0]
+}*/
+
+function ftStep(fs : FtState, op : Op) : opt<FtState>
+requires forall t,u : int :: t in fs.ts && u in fs.ts && u != t ==> fs.ts[u][t] < fs.ts[t][t]
+{
+	match op
+	case Write(tid, loc) => if(tid !in fs.ts && loc !in fs.vs) then Just(FtState(map[tid := map[tid := 1]], map[loc := Epoch(tid,0)],fs.ls)) 
+	else if (tid !in fs.ts) then Nothing
+	else if (tid in fs.ts && loc !in fs.vs) then var oldVal := fs.ts[tid][tid];  
+	
+	
+	//update ts
+	var tmap := fs.ts;
+	var tvc := tmap[tid]; 
+	var tval := tvc[tid] + 1;
+	var tvc := tvc[tid := tval];
+	var tmap := tmap [ tid := tvc];
+	Just(FtState(tmap,map[loc := Epoch(tid,0)],fs.ls))
+	else Nothing	
+	//var eid := if(tid !in fs.ts) then           //fs.vs[loc].tid; 
+	//if(fs.vs[loc].val > fs.ts[tid][eid]) then Nothing else Just(fs)
+} 
+
+
+
+/*ghost method getEmptyVc ( numberOfThreads : nat ) returns ( res : VC )
+requires numberOfThreads > 0
+ensures |res| == numberOfThreads
+ensures forall i : int :: 0 <= i < numberOfThreads ==> res[i] == 0;
+{
+			var k := 0;
+			res := [];
+			while( k < numberOfThreads)
+			invariant k == |res|
+			invariant numberOfThreads >= k >= 0
+			invariant forall i : int :: 0 <= i < k ==> res[i] == 0;
+			
+			{
+				res := [0] + res;
+				k := k + 1;
+			}
+}*/
+/*ghost method initThreadMap(numberOfThreads : nat) returns (res : ThreadsMap)
+ensures forall i:int :: i in res ==> |res[i]| == numberOfThreads;
+ensures forall i: int :: i in res ==> forall j : int :: 0 <= j < numberOfThreads ==> res[i][j] == 0
+ensures forall i:int :: i in res <==> 0 <= i < numberOfThreads
+ensures |res| == numberOfThreads
+{
+	var j := 0;
+	var tmap : ThreadsMap := map[];
+	while( j < numberOfThreads )
+	invariant numberOfThreads >= j >= 0  
+	invariant forall i:int :: i in tmap ==> |tmap[i]| == numberOfThreads;
+	invariant |tmap| == j;
+	invariant forall i:int :: i in tmap <==> 0 <= i < j
+	invariant forall i : int :: i in tmap ==> forall j : int :: 0 <= j < numberOfThreads ==> tmap[i][j] == 0
+	{
+		var vc := getEmptyVc(numberOfThreads);
+        tmap := tmap[j := vc];
+		j := j + 1;
+	}
+	res := tmap;
+}*/
+
+
+
+
+
+
+
+
+function getMaxIdF(t : Trace) : int
+{
+	if(|t| == 0) then 0
+	else 1
+	//else max(t[0].tid, getMaxIdF(t[1..])) 
+}
+
